wip: Binop support

Source/DafnyCompilers/CSharp/Compiler.dfy
@@ -1,5 +1,6 @@
 include "../CSharpDafnyASTModel.dfy"
 include "../CSharpInterop.dfy"
+include "../CSharpDafnyInterop.dfy"
 include "../Library.dfy"
 
 module {:extern "DafnyInDafny.CSharp"} CSharpDafnyCompiler {
@@ -16,22 +17,60 @@ module {:extern "DafnyInDafny.CSharp"} CSharpDafnyCompiler {
     datatype Tokd<T> =
       Tokd(tok: Boogie.IToken, val: T)
 
+    module BinaryOp {
+      datatype Logical =
+        Iff | Imp | And | Or
+      datatype Eq =
+        EqCommon | NeqCommon
+      datatype Numeric =
+        Lt | Le | Ge | Gt | Add | Sub | Mul | Div | Mod
+      datatype BV =
+        LeftShift | RightShift | BitwiseAnd | BitwiseOr | BitwiseXor
+      datatype Char =
+        LtChar | LeChar | GeChar | GtChar
+      datatype Sets =
+        SetEq | SetNeq | ProperSubset | Subset | Superset | ProperSuperset |
+        Disjoint | InSet | NotInSet | Union | Intersection | SetDifference
+      datatype MultiSets =
+        MultiSetEq | MultiSetNeq | MultiSubset | MultiSuperset |
+        ProperMultiSubset | ProperMultiSuperset | MultiSetDisjoint | InMultiSet |
+        NotInMultiSet | MultiSetUnion | MultiSetIntersection | MultiSetDifference
+      datatype Sequences =
+        SeqEq | SeqNeq | ProperPrefix | Prefix | Concat | InSeq | NotInSeq
+      datatype Maps =
+        MapEq | MapNeq | InMap | NotInMap | MapMerge | MapSubtraction
+      datatype Datatypes =
+        RankLt | RankGt
+      datatype Op =
+        | Logical(oLogical: Logical)
+        | Eq(oEq: Eq)
+        | Numeric(oNumeric: Numeric)
+        | BV(oBV: BV)
+        | Char(oChar: Char)
+        | Sets(oSets: Sets)
+        | MultiSets(oMultiSets: MultiSets)
+        | Sequences(oSequences: Sequences)
+        | Maps(oMaps: Maps)
+        | Datatypes(oDatatypes: Datatypes)
+    }
+
     // public class LiteralExpr : Expression
     datatype LiteralExpr =
       | LitBool(b: bool)
       | LitInt(i: int)
       | LitReal(r: real)
       | LitChar(c: string) // FIXME should this use a char?
-      | LitString(s: string)
+      | LitString(s: string, verbatim: bool)
 
-    datatype Expression =
+    datatype Expr =
+      | BinaryExpr(op: BinaryOp.Op, e0: Expr, e1: Expr)
       | LiteralExpr(lit: LiteralExpr)
       | InvalidExpr(msg: string)
       | UnsupportedExpr(expr: C.Expression)
 
     datatype Stmt =
-      | PrintStmt(exprs: seq<Expression>)
-      | InvalidStmt
+      | PrintStmt(exprs: seq<Expr>)
+      | UnsupportedStmt
 
     type BlockStmt = seq<Stmt>
 
@@ -49,51 +88,80 @@ module {:extern "DafnyInDafny.CSharp"} CSharpDafnyCompiler {
     import C = CSharpDafnyASTModel
     import D = AST
 
-    // function method TranslateExpression(c: C.Expression) : D.Expression reads * {
-    //   match c {
-    //   case c: C.LiteralExpr =>
-    //     match c.Value {
-    //     case s: System.String =>
-    //       var str := StringUtils.OfCString(s);
-    //       match c {
-    //       case c: C.CharLiteralExpr =>
-    //         D.LiteralExpr(D.LitChar(str))
-    //       case c: C.StringLiteralExpr =>
-    //         D.LiteralExpr(D.LitString(str))
-    //       case _ =>
-    //         D.InvalidExpr("LiteralExpr with .Value of type string must be a char or a string.")
-    //       }
-    //     case _ => D.UnsupportedExpr(c)
-    //     }
-    //   case _ => D.UnsupportedExpr(c)
-    //   }
-    // }
+    const BinaryOpCodeMap: map<C.BinaryExpr__ResolvedOpcode, D.BinaryOp.Op> :=
+      map[C.BinaryExpr__ResolvedOpcode.Iff := D.BinaryOp.Logical(D.BinaryOp.Iff)]
+         [C.BinaryExpr__ResolvedOpcode.Imp := D.BinaryOp.Logical(D.BinaryOp.Imp)]
+         [C.BinaryExpr__ResolvedOpcode.And := D.BinaryOp.Logical(D.BinaryOp.And)]
+         [C.BinaryExpr__ResolvedOpcode.Or := D.BinaryOp.Logical(D.BinaryOp.Or)]
+         [C.BinaryExpr__ResolvedOpcode.EqCommon := D.BinaryOp.Eq(D.BinaryOp.EqCommon)]
+         [C.BinaryExpr__ResolvedOpcode.NeqCommon := D.BinaryOp.Eq(D.BinaryOp.NeqCommon)]
+         [C.BinaryExpr__ResolvedOpcode.Lt := D.BinaryOp.Numeric(D.BinaryOp.Lt)]
+         [C.BinaryExpr__ResolvedOpcode.Le := D.BinaryOp.Numeric(D.BinaryOp.Le)]
+         [C.BinaryExpr__ResolvedOpcode.Ge := D.BinaryOp.Numeric(D.BinaryOp.Ge)]
+         [C.BinaryExpr__ResolvedOpcode.Gt := D.BinaryOp.Numeric(D.BinaryOp.Gt)]
+         [C.BinaryExpr__ResolvedOpcode.Add := D.BinaryOp.Numeric(D.BinaryOp.Add)]
+         [C.BinaryExpr__ResolvedOpcode.Sub := D.BinaryOp.Numeric(D.BinaryOp.Sub)]
+         [C.BinaryExpr__ResolvedOpcode.Mul := D.BinaryOp.Numeric(D.BinaryOp.Mul)]
+         [C.BinaryExpr__ResolvedOpcode.Div := D.BinaryOp.Numeric(D.BinaryOp.Div)]
+         [C.BinaryExpr__ResolvedOpcode.Mod := D.BinaryOp.Numeric(D.BinaryOp.Mod)]
+         [C.BinaryExpr__ResolvedOpcode.LeftShift := D.BinaryOp.BV(D.BinaryOp.LeftShift)]
+         [C.BinaryExpr__ResolvedOpcode.RightShift := D.BinaryOp.BV(D.BinaryOp.RightShift)]
+         [C.BinaryExpr__ResolvedOpcode.BitwiseAnd := D.BinaryOp.BV(D.BinaryOp.BitwiseAnd)]
+         [C.BinaryExpr__ResolvedOpcode.BitwiseOr := D.BinaryOp.BV(D.BinaryOp.BitwiseOr)]
+         [C.BinaryExpr__ResolvedOpcode.BitwiseXor := D.BinaryOp.BV(D.BinaryOp.BitwiseXor)]
+         [C.BinaryExpr__ResolvedOpcode.LtChar := D.BinaryOp.Char(D.BinaryOp.LtChar)]
+         [C.BinaryExpr__ResolvedOpcode.LeChar := D.BinaryOp.Char(D.BinaryOp.LeChar)]
+         [C.BinaryExpr__ResolvedOpcode.GeChar := D.BinaryOp.Char(D.BinaryOp.GeChar)]
+         [C.BinaryExpr__ResolvedOpcode.GtChar := D.BinaryOp.Char(D.BinaryOp.GtChar)]
+         [C.BinaryExpr__ResolvedOpcode.SetEq := D.BinaryOp.Sets(D.BinaryOp.SetEq)]
+         [C.BinaryExpr__ResolvedOpcode.SetNeq := D.BinaryOp.Sets(D.BinaryOp.SetNeq)]
+         [C.BinaryExpr__ResolvedOpcode.ProperSubset := D.BinaryOp.Sets(D.BinaryOp.ProperSubset)]
+         [C.BinaryExpr__ResolvedOpcode.Subset := D.BinaryOp.Sets(D.BinaryOp.Subset)]
+         [C.BinaryExpr__ResolvedOpcode.Superset := D.BinaryOp.Sets(D.BinaryOp.Superset)]
+         [C.BinaryExpr__ResolvedOpcode.ProperSuperset := D.BinaryOp.Sets(D.BinaryOp.ProperSuperset)]
+         [C.BinaryExpr__ResolvedOpcode.Disjoint := D.BinaryOp.Sets(D.BinaryOp.Disjoint)]
+         [C.BinaryExpr__ResolvedOpcode.InSet := D.BinaryOp.Sets(D.BinaryOp.InSet)]
+         [C.BinaryExpr__ResolvedOpcode.NotInSet := D.BinaryOp.Sets(D.BinaryOp.NotInSet)]
+         [C.BinaryExpr__ResolvedOpcode.Union := D.BinaryOp.Sets(D.BinaryOp.Union)]
+         [C.BinaryExpr__ResolvedOpcode.Intersection := D.BinaryOp.Sets(D.BinaryOp.Intersection)]
+         [C.BinaryExpr__ResolvedOpcode.SetDifference := D.BinaryOp.Sets(D.BinaryOp.SetDifference)]
+         [C.BinaryExpr__ResolvedOpcode.MultiSetEq := D.BinaryOp.MultiSets(D.BinaryOp.MultiSetEq)]
+         [C.BinaryExpr__ResolvedOpcode.MultiSetNeq := D.BinaryOp.MultiSets(D.BinaryOp.MultiSetNeq)]
+         [C.BinaryExpr__ResolvedOpcode.MultiSubset := D.BinaryOp.MultiSets(D.BinaryOp.MultiSubset)]
+         [C.BinaryExpr__ResolvedOpcode.MultiSuperset := D.BinaryOp.MultiSets(D.BinaryOp.MultiSuperset)]
+         [C.BinaryExpr__ResolvedOpcode.ProperMultiSubset := D.BinaryOp.MultiSets(D.BinaryOp.ProperMultiSubset)]
+         [C.BinaryExpr__ResolvedOpcode.ProperMultiSuperset := D.BinaryOp.MultiSets(D.BinaryOp.ProperMultiSuperset)]
+         [C.BinaryExpr__ResolvedOpcode.MultiSetDisjoint := D.BinaryOp.MultiSets(D.BinaryOp.MultiSetDisjoint)]
+         [C.BinaryExpr__ResolvedOpcode.InMultiSet := D.BinaryOp.MultiSets(D.BinaryOp.InMultiSet)]
+         [C.BinaryExpr__ResolvedOpcode.NotInMultiSet := D.BinaryOp.MultiSets(D.BinaryOp.NotInMultiSet)]
+         [C.BinaryExpr__ResolvedOpcode.MultiSetUnion := D.BinaryOp.MultiSets(D.BinaryOp.MultiSetUnion)]
+         [C.BinaryExpr__ResolvedOpcode.MultiSetIntersection := D.BinaryOp.MultiSets(D.BinaryOp.MultiSetIntersection)]
+         [C.BinaryExpr__ResolvedOpcode.MultiSetDifference := D.BinaryOp.MultiSets(D.BinaryOp.MultiSetDifference)]
+         [C.BinaryExpr__ResolvedOpcode.SeqEq := D.BinaryOp.Sequences(D.BinaryOp.SeqEq)]
+         [C.BinaryExpr__ResolvedOpcode.SeqNeq := D.BinaryOp.Sequences(D.BinaryOp.SeqNeq)]
+         [C.BinaryExpr__ResolvedOpcode.ProperPrefix := D.BinaryOp.Sequences(D.BinaryOp.ProperPrefix)]
+         [C.BinaryExpr__ResolvedOpcode.Prefix := D.BinaryOp.Sequences(D.BinaryOp.Prefix)]
+         [C.BinaryExpr__ResolvedOpcode.Concat := D.BinaryOp.Sequences(D.BinaryOp.Concat)]
+         [C.BinaryExpr__ResolvedOpcode.InSeq := D.BinaryOp.Sequences(D.BinaryOp.InSeq)]
+         [C.BinaryExpr__ResolvedOpcode.NotInSeq := D.BinaryOp.Sequences(D.BinaryOp.NotInSeq)]
+         [C.BinaryExpr__ResolvedOpcode.MapEq := D.BinaryOp.Maps(D.BinaryOp.MapEq)]
+         [C.BinaryExpr__ResolvedOpcode.MapNeq := D.BinaryOp.Maps(D.BinaryOp.MapNeq)]
+         [C.BinaryExpr__ResolvedOpcode.InMap := D.BinaryOp.Maps(D.BinaryOp.InMap)]
+         [C.BinaryExpr__ResolvedOpcode.NotInMap := D.BinaryOp.Maps(D.BinaryOp.NotInMap)]
+         [C.BinaryExpr__ResolvedOpcode.MapMerge := D.BinaryOp.Maps(D.BinaryOp.MapMerge)]
+         [C.BinaryExpr__ResolvedOpcode.MapSubtraction := D.BinaryOp.Maps(D.BinaryOp.MapSubtraction)]
+         [C.BinaryExpr__ResolvedOpcode.RankLt := D.BinaryOp.Datatypes(D.BinaryOp.RankLt)]
+         [C.BinaryExpr__ResolvedOpcode.RankGt := D.BinaryOp.Datatypes(D.BinaryOp.RankGt)];
 
-    // function method TranslateExpression'(c: C.Expression) : D.Expression reads * {
-    //   match c {
-    //   | c: C.LiteralExpr =>
-    //     match c.Value {
-    //     | s: System.String =>
-    //       var str := StringUtils.OfCString(s);
-    //       match c {
-    //       | c: C.CharLiteralExpr =>
-    //         D.LiteralExpr(D.LitChar(str))
-    //       | c: C.StringLiteralExpr =>
-    //         D.LiteralExpr(D.LitString(str))
-    //       | _ =>
-    //         D.InvalidExpr("LiteralExpr with .Value of type string must be a char or a string.")
-    //       }
-    //     | _ => D.UnsupportedExpr(c)
-    //     }
-    //   | _ => D.UnsupportedExpr(c)
-    //   }
-    // }
+    function method {:verify false} TranslateBinary(b: C.BinaryExpr) : D.Expr {
+      var op, e0, e1 := b.ResolvedOp, b.E0, b.E1;
+      // LATER b.AccumulatesForTailRecursion
+      assume op in BinaryOpCodeMap.Keys; // FIXME expect
+      D.BinaryExpr(BinaryOpCodeMap[op], TranslateExpression(e0), TranslateExpression(e1))
+    }
 
-    function method TranslateExpression(c: C.Expression) : D.Expression reads * {
-      if c is C.LiteralExpr then
-        var l: C.LiteralExpr := c as C.LiteralExpr;
-
-        if l.Value is System.Boolean then
+    function method TranslateLiteral(l: C.LiteralExpr): D.Expr reads * {
+        if l.Value is Boolean then
           D.LiteralExpr(D.LitBool(TypeConv.AsBool(l.Value)))
         else if l.Value is Numerics.BigInteger then
           D.LiteralExpr(D.LitInt(TypeConv.AsInt(l.Value)))
@@ -104,10 +172,18 @@ module {:extern "DafnyInDafny.CSharp"} CSharpDafnyCompiler {
           if l is C.CharLiteralExpr then
             D.LiteralExpr(D.LitChar(str))
           else if l is C.StringLiteralExpr then
-            D.LiteralExpr(D.LitString(str))
+            var sl := l as C.StringLiteralExpr;
+            D.LiteralExpr(D.LitString(str, sl.IsVerbatim))
           else
             D.InvalidExpr("LiteralExpr with .Value of type string must be a char or a string.")
         else D.UnsupportedExpr(l)
+    }
+
+    function method {:verify false} TranslateExpression(c: C.Expression) : D.Expr reads * {
+      if c is C.BinaryExpr then
+        TranslateBinary(c as C.BinaryExpr)
+      else if c is C.LiteralExpr then
+        TranslateLiteral(c as C.LiteralExpr)
       else D.UnsupportedExpr(c)
     }
 
@@ -115,7 +191,7 @@ module {:extern "DafnyInDafny.CSharp"} CSharpDafnyCompiler {
       if s is C.PrintStmt then
         var p := s as C.PrintStmt;
         D.PrintStmt(Seq.Map(TranslateExpression, ListUtils.ToSeq(p.Args)))
-      else D.InvalidStmt
+      else D.UnsupportedStmt
     }
 
     function method TranslateBlock(b: C.BlockStmt) : D.BlockStmt reads * {
@@ -138,7 +214,7 @@ module {:extern "DafnyInDafny.CSharp"} CSharpDafnyCompiler {
     datatype StrTree =
       | Str(s: string)
       | SepSeq(sep: Option<string>, asts: seq<StrTree>)
-      | Invalid
+      | Unsupported
 
     function method Seq(asts: seq<StrTree>) : StrTree {
       SepSeq(None, asts)
@@ -159,6 +235,82 @@ module {:extern "DafnyInDafny.CSharp"} CSharpDafnyCompiler {
     function method DoubleQuote(s: StrTree): StrTree {
       Seq([Str("\""), s, Str("\"")])
     }
+
+    function method interleave<T>(t0: seq<T>, t1: seq<T>, pos: int) : seq<T>
+      requires 0 <= pos
+      requires pos <= |t0| && pos <= |t1|
+      decreases |t0| - pos
+    {
+      if pos >= |t1| then t0[pos..]
+      else if pos >= |t0| then t1[pos..]
+      else [t0[pos], t1[pos]] + interleave(t0, t1, pos + 1)
+    }
+
+
+    function method splitFormat'(formatString: string, prev: int, pos: int) : (parts: seq<StrTree>)
+      requires 0 <= prev <= pos <= |formatString|
+      ensures |parts| > 0
+      decreases |formatString| - pos
+    {
+      if pos >= |formatString| - 1 then
+        [Str(formatString[prev..])]
+      else if formatString[pos] == '{' && formatString[pos + 1] == '}' then
+        [Str(formatString[prev..pos])] + splitFormat'(formatString, pos + 2, pos + 2)
+      else
+        splitFormat'(formatString, prev, pos + 1)
+    }
+
+    function method splitFormat(formatString: string) : seq<StrTree> {
+      splitFormat'(formatString, 0, 0)
+    }
+
+    function method Format(s: string, values: seq<StrTree>): StrTree
+      requires |splitFormat(s)| == |values| + 1
+    {
+      Seq(interleave(splitFormat(s), values, 0))
+    }
+  }
+
+  module Rewriter {
+    import Lib
+    import opened AST
+    import opened Target
+    import opened Lib.Datatypes
+    import opened CSharpInterop
+
+    module MapExprs {
+      import opened Lib
+      import opened AST
+
+      function method MapExprs_Stmt(s: Stmt, f: Expr -> Expr) : Stmt {
+        match s {
+          case PrintStmt(exprs) =>
+            PrintStmt(Seq.Map(f, exprs))
+          case UnsupportedStmt => s
+        }
+      }
+
+      function method MapExprs_BlockStmt(b: BlockStmt, f: Expr -> Expr) : BlockStmt {
+        Seq.Map((s => MapExprs_Stmt(s, f)), b)
+      }
+
+      function method MapExprs_Method(m: Method, f: Expr -> Expr) : Method {
+        match m {
+          case Method(CompileName, methodBody) =>
+            Method(CompileName, MapExprs_BlockStmt(methodBody, f))
+        }
+      }
+
+      function method MapExprs_Program(p: Program, f: Expr -> Expr) : Program {
+        match p {
+          case Program(mainMethod) => Program(MapExprs_Method(mainMethod, f))
+        }
+      }
+
+      function method MapExprs(p: Program, f: Expr -> Expr) : Program {
+        MapExprs_Program(p, f)
+      }
+    }
   }
 
   module Compiler {
@@ -174,32 +326,126 @@ module {:extern "DafnyInDafny.CSharp"} CSharpDafnyCompiler {
       Call("new BigInteger", [Str(istr)])
     }
 
-    function method CompileExpression(s: Expression) : StrTree {
-      match s {
-        case LiteralExpr(l) =>
-          match l {
-            case LitBool(b: bool) => Str(if b then "true" else "false")
-            case LitInt(i: int) => CompileInt(i)
-            case LitReal(r: real) =>
-              var n := TypeConv.Numerator(r);
-              var d := TypeConv.Denominator(r);
-              Call("new BigRational", [CompileInt(n), CompileInt(d)])
-            case LitChar(c: string) => SingleQuote(Str(c))
-            case LitString(s: string) => DoubleQuote(Str(s))
-          }
-        case InvalidExpr => Invalid
+    function method CompileLiteralExpr(l: LiteralExpr) : StrTree {
+      match l {
+        case LitBool(b: bool) => Str(if b then "true" else "false")
+        case LitInt(i: int) => CompileInt(i)
+        case LitReal(r: real) =>
+          var n := TypeConv.Numerator(r);
+          var d := TypeConv.Denominator(r);
+          Call("new BigRational", [CompileInt(n), CompileInt(d)])
+        case LitChar(c: string) => SingleQuote(Str(c))
+        case LitString(s: string, verbatim: bool) => DoubleQuote(Str(s)) // FIXME verbatim
       }
     }
 
-    function method CompilePrint(e: Expression) : StrTree {
-      Seq([Call("DafnyRuntime.Helpers.Print", [CompileExpression(e)]), Str(";")])
+    // NEXT: Write a transformation that translates negations into unary op + unnegated binary op, apply it using the expr mapper, then write a predicate on the AST that rules out negated exprs, and finally omit the relevant cases from CompileBinaryExpr below.
+
+    function method CompileBinaryExpr(op: BinaryOp.Op, c0: StrTree, c1: StrTree) : StrTree {
+      var fmt := str requires |splitFormat(str)| == 3 =>
+        Format(str, [c0, c1]); // Cute use of function precondition
+      var bin := str =>
+        Format("{} {} {}", [c0, Str(str), c1]);
+      var rbin := str =>
+        Format("{} {} {}", [c1, Str(str), c0]);
+      match op {
+        case Logical(Iff) => bin("==")
+        case Logical(Imp) => fmt("!{} || {}")
+        case Logical(And) => bin("&&")
+        case Logical(Or) => bin("||")
+
+        case Eq(EqCommon) => Unsupported
+        case Eq(NeqCommon) => Unsupported
+
+        case Numeric(Lt) => bin("<")
+        case Numeric(Le) => bin("<=")
+        case Numeric(Ge) => bin(">=")
+        case Numeric(Gt) => bin(">")
+        case Numeric(Add) => Unsupported
+        case Numeric(Sub) => Unsupported
+        case Numeric(Mul) => Unsupported
+        case Numeric(Div) => Unsupported
+        case Numeric(Mod) => Unsupported
+
+        case BV(LeftShift) => Unsupported
+        case BV(RightShift) => Unsupported
+        case BV(BitwiseAnd) => bin("&")
+        case BV(BitwiseOr) => bin("|")
+        case BV(BitwiseXor) => bin("^")
+
+        case Char(LtChar) => bin("<")
+        case Char(LeChar) => bin("<=")
+        case Char(GeChar) => bin(">=")
+        case Char(GtChar) => bin(">")
+        // FIXME: Why is there lt/le/gt/ge for chars but not binops?
+
+        case Sets(SetEq) => fmt("{}.Equals({})")
+        case Sets(SetNeq) => Unsupported
+        case Sets(ProperSubset) => Unsupported
+        case Sets(Subset) => Unsupported
+        case Sets(Superset) => Unsupported
+        case Sets(ProperSuperset) => Unsupported
+        case Sets(Disjoint) => Unsupported
+        case Sets(InSet) => rbin("{}.Contains({})")
+        case Sets(NotInSet) => Unsupported
+        case Sets(Union) => Unsupported
+        case Sets(Intersection) => Unsupported
+        case Sets(SetDifference) => Unsupported
+
+        case MultiSets(MultiSetEq) => fmt("{}.Equals({})")
+        case MultiSets(MultiSetNeq) => Unsupported
+        case MultiSets(MultiSubset) => Unsupported
+        case MultiSets(MultiSuperset) => Unsupported
+        case MultiSets(ProperMultiSubset) => Unsupported
+        case MultiSets(ProperMultiSuperset) => Unsupported
+        case MultiSets(MultiSetDisjoint) => Unsupported
+        case MultiSets(InMultiSet) => rbin("{}.Contains({})")
+        case MultiSets(NotInMultiSet) => Unsupported
+        case MultiSets(MultiSetUnion) => Unsupported
+        case MultiSets(MultiSetIntersection) => Unsupported
+        case MultiSets(MultiSetDifference) => Unsupported
+
+        case Sequences(SeqEq) => fmt("{}.Equals({})")
+        case Sequences(SeqNeq) => Unsupported
+        case Sequences(ProperPrefix) => Unsupported
+        case Sequences(Prefix) => Unsupported
+        case Sequences(Concat) => Unsupported
+        case Sequences(InSeq) => Unsupported
+        case Sequences(NotInSeq) => Unsupported
+
+        case Maps(MapEq) => fmt("{}.Equals({})")
+        case Maps(MapNeq) => Unsupported
+        case Maps(InMap) => rbin("{}.Contains({})")
+        case Maps(NotInMap) => Unsupported
+        case Maps(MapMerge) => Unsupported
+        case Maps(MapSubtraction) => Unsupported
+
+        case Datatypes(RankLt) => Unsupported
+        case Datatypes(RankGt) => Unsupported
+      }
+    }
+
+    function method CompileExpr(s: Expr) : StrTree {
+      match s {
+        case LiteralExpr(l) =>
+          CompileLiteralExpr(l)
+        case BinaryExpr(op, e0, e1) =>
+          var c0, c1 := CompileExpr(e0), CompileExpr(e1);
+          CompileBinaryExpr(op, c0, c1)
+        case InvalidExpr(_) => Unsupported
+        case UnsupportedExpr(_) => Unsupported
+      }
+    }
+
+    function method CompilePrint(e: Expr) : StrTree {
+      Seq([Call("DafnyRuntime.Helpers.Print", [CompileExpr(e)]), Str(";")])
     }
 
     function method CompileStmt(s: Stmt) : StrTree {
       match s {
         case PrintStmt(exprs) =>
           Concat("\n", Lib.Seq.Map(CompilePrint, exprs))
-        case InvalidStmt => Invalid
+        case UnsupportedStmt => Unsupported
       }
     }
 
@@ -216,7 +462,7 @@ module {:extern "DafnyInDafny.CSharp"} CSharpDafnyCompiler {
     }
   }
 
-  method WriteAST(wr: SyntaxTreeAdapter, ast: Target.StrTree) {
+  method WriteAST(wr: CSharpDafnyInterop.SyntaxTreeAdapter, ast: Target.StrTree) {
     match ast {
       case Str(s) =>
         wr.Write(s);
@@ -227,7 +473,7 @@ module {:extern "DafnyInDafny.CSharp"} CSharpDafnyCompiler {
           }
           WriteAST(wr, asts[i]);
         }
-      case Invalid =>
+      case Unsupported =>
     }
   }
 
@@ -237,7 +483,7 @@ module {:extern "DafnyInDafny.CSharp"} CSharpDafnyCompiler {
 
     method Compile(dafnyProgram: CSharpDafnyASTModel.Program,
                    wr: ConcreteSyntaxTree) {
-      var st := new SyntaxTreeAdapter(wr);
+      var st := new CSharpDafnyInterop.SyntaxTreeAdapter(wr);
       var translated := Translator.TranslateProgram(dafnyProgram);
       var compiled := Compiler.CompileProgram(translated);
       WriteAST(st, compiled);
